thy/Primitive_Matchers/Primitive_Abstract.thy
@@ -17,17 +17,30 @@ text\<open>Abstract over certain primitives. The first parameter is a function
 \<close>
 (*TODO: damn tosting function!*)
 fun abstract_primitive
-  :: "(32 common_primitive negation_type \<Rightarrow> bool) \<Rightarrow> 32 common_primitive match_expr \<Rightarrow> 32 common_primitive match_expr" where
+  :: "('i::len common_primitive negation_type \<Rightarrow> bool) \<Rightarrow> 'i common_primitive match_expr \<Rightarrow> 'i common_primitive match_expr"
+where
   "abstract_primitive _     MatchAny = MatchAny" |
-  "abstract_primitive disc (Match a) = (if disc (Pos a) then Match (Extra (common_primitive_v4_toString a)) else (Match a))" |
-  "abstract_primitive disc (MatchNot (Match a)) = (if disc (Neg a) then Match (Extra (''! ''@common_primitive_v4_toString a)) else (MatchNot (Match a)))" |
+  "abstract_primitive disc (Match a) =
+      (if
+         disc (Pos a)
+       then
+         Match (Extra (common_primitive_toString ipaddr_generic_toString a))
+       else
+         (Match a))" |
+  "abstract_primitive disc (MatchNot (Match a)) =
+      (if
+         disc (Neg a)
+       then
+         Match (Extra (''! ''@common_primitive_toString ipaddr_generic_toString a))
+       else
+         (MatchNot (Match a)))" |
   "abstract_primitive disc (MatchNot m) = MatchNot (abstract_primitive disc m)" |
   "abstract_primitive disc (MatchAnd m1 m2) = MatchAnd (abstract_primitive disc m1) (abstract_primitive disc m2)"
 
 
 text\<open>For example, a simple firewall requires that no negated interfaces and protocols occur in the 
       expression.\<close>
-definition abstract_for_simple_firewall :: "32 common_primitive match_expr \<Rightarrow> 32 common_primitive match_expr"
+definition abstract_for_simple_firewall :: "'i::len common_primitive match_expr \<Rightarrow> 'i common_primitive match_expr"
   where "abstract_for_simple_firewall \<equiv> abstract_primitive (\<lambda>r. case r
                 of Pos a \<Rightarrow> is_CT_State a \<or> is_L4_Flags a
                 |  Neg a \<Rightarrow> is_Iiface a \<or> is_Oiface a \<or> is_Prot a \<or> is_CT_State a \<or> is_L4_Flags a)"
@@ -65,19 +78,19 @@ lemma not_hasdisc_ctstate_assume_state: "\<not> has_disc is_CT_State (ctstate_as
   by(induction m rule: ctstate_assume_state.induct) (simp_all)
 
 
-lemma abstract_for_simple_firewall_hasdisc:
-  "\<not> has_disc is_CT_State (abstract_for_simple_firewall m)"
-  "\<not> has_disc is_L4_Flags (abstract_for_simple_firewall m)"
+lemma abstract_for_simple_firewall_hasdisc: fixes m :: "'i::len common_primitive match_expr"
+  shows "\<not> has_disc is_CT_State (abstract_for_simple_firewall m)"
+  and   "\<not> has_disc is_L4_Flags (abstract_for_simple_firewall m)"
   unfolding abstract_for_simple_firewall_def
-  apply(induction "(\<lambda>r:: 32 common_primitive negation_type. case r of Pos a \<Rightarrow> is_CT_State a | Neg a \<Rightarrow> is_Iiface a \<or> is_Oiface a \<or> is_Prot a \<or> is_CT_State a)" m rule: abstract_primitive.induct)
+  apply(induction "(\<lambda>r:: 'i common_primitive negation_type. case r of Pos a \<Rightarrow> is_CT_State a | Neg a \<Rightarrow> is_Iiface a \<or> is_Oiface a \<or> is_Prot a \<or> is_CT_State a)" m rule: abstract_primitive.induct)
   apply(simp_all)
   done
 
-lemma abstract_for_simple_firewall_negated_ifaces_prots:
-    "normalized_nnf_match m \<Longrightarrow> \<not> has_disc_negated (\<lambda>a. is_Iiface a \<or> is_Oiface a) False (abstract_for_simple_firewall m)"
-    "normalized_nnf_match m \<Longrightarrow> \<not> has_disc_negated is_Prot False (abstract_for_simple_firewall m)"
+lemma abstract_for_simple_firewall_negated_ifaces_prots: fixes m :: "'i::len common_primitive match_expr"
+  shows  "normalized_nnf_match m \<Longrightarrow> \<not> has_disc_negated (\<lambda>a. is_Iiface a \<or> is_Oiface a) False (abstract_for_simple_firewall m)"
+  and "normalized_nnf_match m \<Longrightarrow> \<not> has_disc_negated is_Prot False (abstract_for_simple_firewall m)"
   unfolding abstract_for_simple_firewall_def
-  apply(induction "(\<lambda>r:: 32 common_primitive negation_type. case r of Pos a \<Rightarrow> is_CT_State a | Neg a \<Rightarrow> is_Iiface a \<or> is_Oiface a \<or> is_Prot a \<or> is_CT_State a)" m rule: abstract_primitive.induct)
+  apply(induction "(\<lambda>r:: 'i common_primitive negation_type. case r of Pos a \<Rightarrow> is_CT_State a | Neg a \<Rightarrow> is_Iiface a \<or> is_Oiface a \<or> is_Prot a \<or> is_CT_State a)" m rule: abstract_primitive.induct)
   apply(simp_all)
   done
 
@@ -118,7 +131,7 @@ begin
      done
   
   theorem abstract_primitive_in_doubt_allow_generic:
-    fixes \<beta>::"(32 common_primitive, (32, 'a) simple_packet_scheme) exact_match_tac"
+    fixes \<beta>::"('i::len common_primitive, ('i, 'a) simple_packet_scheme) exact_match_tac"
     assumes generic: "primitive_matcher_generic \<beta>"
        and n: "\<forall> m \<in> get_match ` set rs. normalized_nnf_match m" and simple: "simple_ruleset rs"
     defines "\<gamma> \<equiv> (\<beta>, in_doubt_allow)" and "abstract disc \<equiv> optimize_matches (abstract_primitive disc)"
@@ -131,8 +144,8 @@ begin
       from optimize_matches_simple_ruleset simple simple_imp_good_ruleset have
        good: "good_ruleset (optimize_matches (abstract_primitive disc) rs)" by fast
 
-      let ?\<gamma>="(\<beta>, in_doubt_allow) :: (32 common_primitive \<Rightarrow> (32, 'a) simple_packet_scheme \<Rightarrow> ternaryvalue) \<times>
-              (action \<Rightarrow> (32, 'a) simple_packet_scheme \<Rightarrow> bool)"
+      let ?\<gamma>="(\<beta>, in_doubt_allow) :: ('i common_primitive \<Rightarrow> ('i, 'a) simple_packet_scheme \<Rightarrow> ternaryvalue) \<times>
+              (('i, 'a) simple_packet_scheme unknown_match_tac)"
         --\<open>type signature is needed, otherwise @{const in_doubt_allow} would be for arbitrary packet\<close>
 
       have abstract_primitive_in_doubt_allow_help1:
@@ -263,7 +276,7 @@ begin
      done
 
   theorem abstract_primitive_in_doubt_deny_generic:
-    fixes \<beta>::"(32 common_primitive, (32, 'a) simple_packet_scheme) exact_match_tac"
+    fixes \<beta>::"('i::len common_primitive, ('i, 'a) simple_packet_scheme) exact_match_tac"
     assumes generic: "primitive_matcher_generic \<beta>"
         and n: "\<forall> m \<in> get_match ` set rs. normalized_nnf_match m" and simple: "simple_ruleset rs"
     defines "\<gamma> \<equiv> (\<beta>, in_doubt_deny)" and "abstract disc \<equiv> optimize_matches (abstract_primitive disc)"
@@ -276,8 +289,7 @@ begin
       from optimize_matches_simple_ruleset simple simple_imp_good_ruleset have
         good: "good_ruleset (optimize_matches (abstract_primitive disc) rs)" by fast
 
-      let ?\<gamma>="(\<beta>, in_doubt_deny) :: (32 common_primitive \<Rightarrow> (32, 'a) simple_packet_scheme \<Rightarrow> ternaryvalue) \<times> 
-            (action \<Rightarrow> (32, 'a) simple_packet_scheme \<Rightarrow> bool)"
+      let ?\<gamma>="(\<beta>, in_doubt_deny) :: ('i::len common_primitive, ('i, 'a) simple_packet_scheme) match_tac"
         --\<open>type signature is needed, otherwise @{const in_doubt_allow} would be for arbitrary packet\<close>
       
       have abstract_primitive_in_doubt_deny_help1:
